pan-shape: begin verification for real
It seems not that much additional effort to just verify the pan-structs pass.

OK, some of the issues about using a sub-shape-construct (dropWhile etc) were
fiddly, but the verification is now handling "eval", except for the part about
deducing the shape of an expression.

pancake/proofs/pan_structsProofScript.sml
@@ -7,7 +7,7 @@
 *)
 Theory pan_structsProof
 Ancestors
-  panSem pan_structs panProps panLang
+  panSem pan_structs panProps panLang pan_commonProps
 Libs
   preamble
 
@@ -31,40 +31,636 @@ Proof
   \\ metis_tac []
 QED
 
-Theorem compile_shape_eq_pre[local]:
-  (!x shape. ss = x /\ is_wf_shape_nil shape ==>
-    compile_shape ss shape = shape) ∧
-  (!x shapes. ss = x /\ EVERY is_wf_shape_nil shapes ==>
-    compile_shapes ss shapes = shapes)
+val sh_ctxt = rand ``SND (compile_shape ctxt.structs, ctxt.structs) = sh_ctxt``;
+val sh_ctxt_ty = type_of sh_ctxt;
+
+Definition convert_v_def:
+  convert_v (Val x) = Val x /\
+  convert_v (RStruct xs) = RStruct (MAP convert_v xs) /\
+  convert_v (NStruct nm flds) = (let
+    vs = MAP (\(nm, v). convert_v v) flds
+  in RStruct vs)
+End
+
+Definition v_flds_ok_def:
+  v_flds_ok _ (Val x) = T /\
+  v_flds_ok sh_ctxt (RStruct vs) = EVERY (v_flds_ok sh_ctxt) vs /\
+  v_flds_ok sh_ctxt (NStruct nm flds) =
+    (EVERY (\(nm, v). v_flds_ok sh_ctxt v) flds /\
+        (case ALOOKUP sh_ctxt nm of NONE => F | SOME flds2 => MAP FST flds = MAP FST flds2)) 
+End
+
+Definition convert_s_def:
+  convert_s s = s with <|
+    locals := FMAP_MAP2 (\(nm, v). convert_v v) s.locals;
+    globals := FMAP_MAP2 (\(nm, v). convert_v v) s.globals;
+    structs := []
+  |>
+End
+
+Definition s_contents_ok_def:
+  s_contents_ok sh_ctxt s = (
+    FEVERY (\(nm, v). v_flds_ok sh_ctxt v) s.locals /\
+    FEVERY (\(nm, v). v_flds_ok sh_ctxt v) s.globals
+  )
+End
+
+Definition is_wf_shape_ctxt_def:
+  is_wf_shape_ctxt [] = T ∧
+  is_wf_shape_ctxt ((nm, flds) :: sh_ctxt) = (
+    EVERY (is_wf_shape sh_ctxt) (MAP SND flds) ∧
+    is_wf_shape_ctxt sh_ctxt
+  )
+End
+
+Definition structs_ok_def:
+  structs_ok sh_ctxt <=>
+    EVERY (\(nm, flds). ALL_DISTINCT (MAP FST flds)) sh_ctxt ∧
+    ALL_DISTINCT (MAP FST sh_ctxt) ∧
+    is_wf_shape_ctxt sh_ctxt
+End
+
+Definition struct_infos_ok_def:
+  struct_infos_ok sh_ctxt <=>
+    EVERY (\(nm, info). ALL_DISTINCT (MAP FST info.fields)) sh_ctxt ∧
+    ALL_DISTINCT (MAP FST sh_ctxt) ∧
+    (!i nm info. i < LENGTH sh_ctxt /\ EL i sh_ctxt = (nm, info) ==>
+        EVERY (is_wf_shape (DROP (i + 1) sh_ctxt)) (MAP SND info.fields)) ∧
+    EVERY (λ(nm,info). info.size = size_of_sh_with_ctxt sh_ctxt
+        (Comb (MAP SND info.fields))) sh_ctxt
+End
+
+Theorem alookup_drop_helper[local]:
+  ALOOKUP (DROP n xs) k = SOME v /\
+  ALL_DISTINCT (MAP FST xs) ==>
+  ~ MEM k (MAP FST (TAKE n xs)) /\ ALOOKUP xs k = SOME v
+Proof
+  cheat
+QED
+
+Theorem size_of_sh_with_ctxt_drop:
+  !sh_ctxt sh. is_wf_shape (DROP n sh_ctxt) sh /\
+  ALL_DISTINCT (MAP FST sh_ctxt) ==>
+  size_of_sh_with_ctxt (DROP n sh_ctxt) sh = size_of_sh_with_ctxt sh_ctxt sh
+Proof
+  recInduct size_of_sh_with_ctxt_ind
+  >> simp [size_of_sh_with_ctxt_def, is_wf_shape_def]
+  >> simp [Cong MAP_CONG, EVERY_MEM]
+  >> simp [SF ETA_ss]
+  >> rw []
+  >> every_case_tac >> fs []
+  >> imp_res_tac alookup_drop_helper
+  >> simp []
+QED
+
+Theorem is_wf_shape_drop:
+  !sh_ctxt sh n. is_wf_shape (DROP n sh_ctxt) sh ==>
+    is_wf_shape sh_ctxt sh
+Proof
+  recInduct is_wf_shape_ind
+  >> simp [is_wf_shape_def, EVERY_MEM]
+  >> rw []
+  >- (
+    metis_tac []
+  )
+  >- (
+    every_case_tac >> fs [] >>
+    qspecl_then [`TAKE n ctxt`, `DROP n ctxt`, `nm`] mp_tac ALOOKUP_APPEND >>
+    simp [] >>
+    simp [option_case_eq]
+  )
+QED
+
+Theorem struct_infos_ok_drop:
+  struct_infos_ok sh_ctxt ==> struct_infos_ok (DROP n sh_ctxt)
+Proof
+  rw [struct_infos_ok_def, EVERY_DROP, MAP_DROP, ALL_DISTINCT_DROP]
+  >- (
+    gs [EL_DROP]
+    >> first_x_assum (drule_at (Pat `EL _ _ = _`))
+    >> simp [DROP_DROP]
+  )
+  >-(
+    gs [EVERY_EL, EL_DROP]
+    >> rw []
+    >> fs [arithmeticTheory.SUB_LEFT_LESS]
+    >> first_x_assum drule
+    >> simp [ELIM_UNCURRY]
+    >> dep_rewrite.DEP_REWRITE_TAC [size_of_sh_with_ctxt_drop]
+    >> simp [is_wf_shape_def]
+    >> rpt (first_x_assum drule)
+    >> simp []
+    >> pairarg_tac >> fs []
+    >> rw [EVERY_EL]
+    >> res_tac
+    >> irule is_wf_shape_drop
+    >> simp [DROP_DROP]
+    >> qexists_tac `n' + 1`
+    >> simp [DROP_DROP]
+  )
+QED
+
+Theorem struct_infos_ok_append:
+  struct_infos_ok (xs ++ ys) ==> struct_infos_ok ys
+Proof
+  rw []
+  >> drule_then (qspec_then `LENGTH xs` mp_tac) struct_infos_ok_drop
+  >> simp [DROP_APPEND2]
+QED
+
+Theorem is_wf_shape_ctxt_drop:
+  !sh_ctxt n. is_wf_shape_ctxt sh_ctxt ==> is_wf_shape_ctxt (DROP n sh_ctxt)
+Proof
+  Induct
+  >> simp [is_wf_shape_ctxt_def]
+  >> Cases_on `n`
+  >> simp [is_wf_shape_ctxt_def, FORALL_PROD]
+QED
+
+Theorem structs_ok_drop:
+  structs_ok sh_ctxt ==> structs_ok (DROP n sh_ctxt)
+Proof
+  rw [structs_ok_def, EVERY_DROP, MAP_DROP, ALL_DISTINCT_DROP,
+    is_wf_shape_ctxt_drop]
+QED
+
+Theorem compile_shape_eq:
+  (! ^sh_ctxt shape. is_wf_shape_nil shape ==>
+    compile_shape sh_ctxt shape = shape) ∧
+  (! ^sh_ctxt shapes. EVERY is_wf_shape_nil shapes ==>
+    compile_shapes sh_ctxt shapes = shapes)
 Proof
   ho_match_mp_tac compile_shape_ind
   \\ simp [compile_shape_def, is_wf_shape_def, SF ETA_ss]
 QED
 
-Theorem compile_shape_eq = Q.GEN `ss` compile_shape_eq_pre |> SIMP_RULE bool_ss []
-
 Theorem compile_exp_correct_mmap_helper[local]:
-  !es vs. OPT_MMAP (\e. eval s e) es = SOME vs /\
-  (!e. MEM e es ==> (!v. eval s e = SOME v ==> eval s (compile_exp ctxt e) = SOME v)) ==>
-  OPT_MMAP (λa. eval s a) (compile_exps ctxt es) = SOME vs
+  !es vs. OPT_MMAP (eval s) es = SOME vs /\
+  (!e. MEM e es ==> (!v. eval s e = SOME v ==>
+    eval (convert_s s) (compile_exp ctxt e) = SOME (convert_v v))) ==>
+  OPT_MMAP (eval (convert_s s)) (compile_exps ctxt es) = SOME (MAP convert_v vs)
 Proof
   Induct
-  \\ simp [compile_exp_def, DISJ_IMP_THM, FORALL_AND_THM]
-  \\ rw []
+  >> simp [compile_exp_def, DISJ_IMP_THM, FORALL_AND_THM]
+  >> rw []
+  >> simp []
 QED
 
-Theorem compile_exp_correct:
-  ∀s e v.
-  eval s e = SOME v ∧
-  s.structs = []
-  ⇒
-  eval s (compile_exp ctxt e) = SOME v
+Theorem fields_in_order_reorder_noop:
+  !eflds info_fields. MAP FST info_fields = MAP FST eflds /\
+  ALL_DISTINCT (MAP FST info_fields) ==>
+  FLAT (MAP (λ(nm',sh). case ALOOKUP (compile_fields ctxt eflds) nm' of
+         NONE => [] | SOME e => [e]) info_fields) =
+  MAP (compile_exp ctxt o SND) eflds
 Proof
+  Induct >>
+  simp [MAP_EQ_CONS, EXISTS_PROD] >>
+  simp [PULL_EXISTS, FORALL_PROD] >>
+  simp [compile_exp_def] >>
+  rw [] >>
+  irule EQ_TRANS >>
+  first_x_assum (irule_at Any) >>
+  simp [] >>
+  irule_at Any EQ_REFL >>
+  simp [] >>
+  AP_TERM_TAC >>
+  irule MAP_CONG >>
+  simp [FORALL_PROD] >>
+  rw [] >>
+  every_case_tac >> fs [] >>
+  gs [MEM_MAP, FORALL_PROD]
+QED
+
+Theorem alookup_map_structs_ok[local]:
+  ALOOKUP s.structs nm = SOME info /\
+  structs_ok (MAP (λ(nm,info). (nm, info.fields)) s.structs) ==>
+  ALL_DISTINCT (MAP FST info.fields)
+Proof
+  rw []
+  >> imp_res_tac ALOOKUP_MEM
+  >> fs [structs_ok_def, EVERY_MAP]
+  >> imp_res_tac EVERY_MEM
+  >> fs []
+QED
+
+Theorem opt_mmap_eq_every[local]:
+  OPT_MMAP f xs = SOME ys /\
+  (!x y. MEM x xs /\ f x = SOME y ==> P y) ==>
+  EVERY P ys
+Proof
+  rw [EVERY_EL]
+  >> imp_res_tac opt_mmap_length_eq >> fs []
+  >> imp_res_tac opt_mmap_el >> fs []
+  >> gs []
+  >> res_tac
+  >> metis_tac [EL_MEM]
+QED
+
+Theorem every_convert_v_eq[local]:
+  EVERY (\w. case w of Val _ => T | _ => F) vs ==>
+  MAP convert_v vs = vs
+Proof
+  rw [EVERY_EL, LIST_EQ_REWRITE]
+  >> res_tac
+  >> every_case_tac
+  >> fs [EL_MAP, convert_v_def]
+QED
+
+Theorem map_fst_eq_alookup[local]:
+  !xs ys. MAP FST xs = MAP FST ys /\
+  ALOOKUP xs nm = SOME v ==>
+  ?i. afindi nm xs = SOME i /\ afindi nm ys = SOME i /\
+    i < LENGTH xs /\ i < LENGTH ys /\
+    v = SND (EL i xs) /\ ALOOKUP ys nm = SOME (SND (EL i ys))
+Proof
+  Induct_on `ys`
+  >> simp [FORALL_PROD, MAP_EQ_CONS, PULL_EXISTS]
+  >> rw []
+  >> simp [afindi_def]
+  >> first_x_assum (drule o GSYM)
+  >> simp []
+  >> disch_then (assume_tac o GSYM)
+  >> fs [EL_CONS, PRE_SUB1]
+QED
+
+Theorem is_wf_shape_nil_compile_shape:
+  (! ^sh_ctxt sh. is_wf_shape_nil (compile_shape sh_ctxt sh))
+  ∧
+  (! ^sh_ctxt shs. EVERY is_wf_shape_nil (compile_shapes sh_ctxt shs))
+Proof
+  ho_match_mp_tac compile_shape_ind
+  >> simp [compile_shape_def, is_wf_shape_def, SF ETA_ss]
+  >> rw []
+  >> every_case_tac
+  >> simp [is_wf_shape_def, SF ETA_ss]
+QED
+
+Theorem compile_shapes_eq_map:
+  !shs. compile_shapes sctxt shs = MAP (compile_shape sctxt) shs
+Proof
+  Induct
+  >> simp [compile_shape_def]
+QED
+
+Theorem mem_load_flds_eq:
+  ! fld_shs vflds x. mem_load_flds fld_shs x madd memry stcs = SOME vflds ==> 
+  ?vs. mem_loads (MAP SND fld_shs) x madd memry stcs = SOME vs /\
+    LENGTH vs = LENGTH fld_shs /\ vflds = ZIP (MAP FST fld_shs, vs)
+Proof
+  Induct
+  >> simp [mem_load_def, FORALL_PROD]
+  >> rpt (gen_tac ORELSE disch_tac)
+  >> gvs [option_case_eq, shape_case_eq]
+  >> first_x_assum drule
+  >> rw []
+  >> simp []
+QED
+
+Theorem ALOOKUP_ALL_DISTINCT_split:
+  ALL_DISTINCT (MAP FST xs) /\ ALOOKUP xs nm = SOME y ==>
+  ?xs1 xs2. xs = xs1 ++ [(nm, y)] ++ xs2 /\
+  ~ MEM nm (MAP FST xs1) /\ ~ MEM nm (MAP FST xs2)
+Proof
+  Induct_on `xs`
+  >> simp [FORALL_PROD]
+  >> rw []
+  >- (
+    qexists_tac `[]`
+    >> simp []
+  )
+  >> fs []
+  >> REWRITE_TAC [GSYM (cj 2 APPEND)]
+  >> irule_at Any EQ_REFL
+  >> simp []
+QED
+
+Theorem ALOOKUP_ALL_DISTINCT_DROP_split:
+  !xs n. ALL_DISTINCT (MAP FST xs) /\ ALOOKUP (DROP n xs) nm = SOME y ==>
+  ?xs1 xs2. xs = xs1 ++ [(nm, y)] ++ xs2 /\
+  n <= LENGTH xs1 /\ ~ MEM nm (MAP FST xs1) /\ ~ MEM nm (MAP FST xs2)
+Proof
+  rw []
+  >> qspecl_then [`TAKE n xs`, `DROP n xs`, `nm`] mp_tac ALOOKUP_APPEND
+  >> simp []
+  >> TOP_CASE_TAC
+  >- (
+    rw []
+    >> drule_then drule ALOOKUP_ALL_DISTINCT_split
+    >> rw []
+    >> irule_at Any EQ_REFL
+    >> simp []
+    >> CCONTR_TAC
+    >> fs [DROP_APPEND, TAKE_APPEND, ALOOKUP_APPEND]
+    >> fs [option_case_eq]
+  )
+  >- (
+    imp_res_tac ALOOKUP_MEM
+    >> fs [MEM_SPLIT]
+    >> qspecl_then [`n`, `xs`] mp_tac TAKE_DROP
+    >> asm_simp_tac bool_ss []
+    >> rw []
+    >> fs [ALL_DISTINCT_APPEND]
+  )
+QED
+
+Theorem size_of_compile_shape_ind[local]:
+  (! ^sh_ctxt sh ctxt n.
+    sh_ctxt = MAP (λ(nm,info). (nm, info.fields)) (DROP n ctxt) /\
+    is_wf_shape (DROP n ctxt) sh /\
+    struct_infos_ok ctxt ==>
+    size_of_sh_with_ctxt [] (compile_shape sh_ctxt sh) = size_of_sh_with_ctxt ctxt sh
+  ) /\
+  (! ^sh_ctxt shs ctxt n.
+    sh_ctxt = MAP (λ(nm,info). (nm, info.fields)) (DROP n ctxt) /\
+    EVERY (is_wf_shape (DROP n ctxt)) shs /\
+    struct_infos_ok ctxt ==>
+    SUM (MAP (size_of_sh_with_ctxt []) (compile_shapes sh_ctxt shs)) =
+      SUM (MAP (size_of_sh_with_ctxt ctxt) shs)
+  )
+Proof
+  ho_match_mp_tac compile_shape_ind
+  >> rw []
+  >> simp [compile_shape_def, size_of_sh_with_ctxt_def]
+  >> fs [SF ETA_ss, is_wf_shape_def]
+  (* one non-trivial case, named shapes *)
+  >> fs [ALOOKUP_MAP]
+  >> Cases_on `ALOOKUP (DROP n ctxt) nm` >> fs []
+  >> imp_res_tac struct_infos_ok_def
+  >> drule_then drule ALOOKUP_ALL_DISTINCT_DROP_split
+  >> strip_tac
+  >> fs [DROP_APPEND1]
+  >> fs [dropWhile_APPEND_EXISTS]
+  >> dep_rewrite.DEP_REWRITE_TAC [dropWhile_APPEND_EVERY]
+  >> conj_asm1_tac
+  >- (
+    simp [EVERY_MAP, ELIM_UNCURRY]
+    >> irule EVERY_DROP
+    >> fs [EVERY_MEM, MEM_MAP]
+    >> metis_tac []
+  )
+  >> fs [dropWhile_APPEND_EVERY]
+  >> simp [size_of_sh_with_ctxt_def]
+  >> simp [ALOOKUP_APPEND, last (RES_CANON ALOOKUP_NONE)]
+  >> simp [size_of_sh_with_ctxt_def, SF ETA_ss]
+  >> irule EQ_TRANS
+  >> last_x_assum (irule_at Any)
+  >> qexists_tac `LENGTH xs1 + 1`
+  >> simp [DROP_APPEND2]
+  >> rfs [struct_infos_ok_def]
+  >> first_x_assum (qspec_then `LENGTH xs1` mp_tac)
+  >> simp [EL_APPEND, DROP_APPEND2]
+QED
+
+Theorem size_of_compile_shape:
+  is_wf_shape ctxt sh /\
+  struct_infos_ok ctxt ==>
+  size_of_sh_with_ctxt [] (compile_shape (MAP (λ(nm,info). (nm, info.fields)) ctxt) sh) =
+    size_of_sh_with_ctxt ctxt sh
+Proof
+  rw []
+  >> irule EQ_TRANS
+  >> drule_at_then Any (irule_at Any) (cj 1 size_of_compile_shape_ind)
+  >> qexists_tac `0`
+  >> simp []
+QED
+
+Theorem dropWhile_MAP_helper:
+  !xs. dropWhile P xs = ys /\
+  (!x. MEM x xs ==> P x = Q (f x)) ==>
+  dropWhile Q (MAP f xs) = MAP f ys
+Proof
+  Induct
+  >> rw []
+  >> gs []
+QED
+
+
+
+val x = ``x : 'a word``
+
+
+Theorem mem_load_conversion:
+  (! str2 shape ^x madd mem str v.
+  mem_load shape x madd mem str = SOME v ∧
+  str2 = MAP (λ(nm,info). (nm,info.fields)) str ∧
+  is_wf_shape str shape ∧
+  struct_infos_ok str ⇒
+  mem_load (compile_shape str2 shape) x madd mem [] = SOME (convert_v v)
+  ) ∧
+  (! str2 shapes ^x madd mem str vs.
+  mem_loads shapes x madd mem str = SOME vs ∧
+  str2 = MAP (λ(nm,info). (nm,info.fields)) str  ∧
+  EVERY (is_wf_shape str) shapes ∧
+  struct_infos_ok str ⇒
+  mem_loads (compile_shapes str2 shapes) x madd mem [] = SOME (MAP convert_v vs)
+  )
+Proof
+  ho_match_mp_tac compile_shape_ind
+  >> rpt conj_tac
+  >> rpt (gen_tac ORELSE disch_tac)
+  >- (
+    gvs [compile_shape_def, mem_load_def, convert_v_def, v_flds_ok_def]
+  )
+  >- (
+    gvs [compile_shape_def, mem_load_def, convert_v_def, v_flds_ok_def,
+        option_case_eq, SF ETA_ss, is_wf_shape_def]
+    >> first_x_assum drule
+    >> simp []
+  )
+  >- (
+    gvs [compile_shape_def, mem_load_def, convert_v_def, v_flds_ok_def,
+        option_case_eq, SF ETA_ss, list_case_eq, pair_case_eq, is_wf_shape_def]
+    >> simp [ALOOKUP_MAP]
+    >> fs [CasePred "option"]
+    >> imp_res_tac struct_infos_ok_def
+    >> drule_then drule ALOOKUP_ALL_DISTINCT_split
+    >> strip_tac
+    >> fs [DROP_APPEND1, dropWhile_APPEND_EXISTS]
+    >> fs [REWRITE_RULE [EVERY_MEM] dropWhile_APPEND_EVERY, MEM_MAP, PULL_EXISTS, FORALL_PROD]
+    >> dep_rewrite.DEP_REWRITE_TAC [REWRITE_RULE [EVERY_MEM] dropWhile_APPEND_EVERY]
+    >> simp [MEM_MAP, PULL_EXISTS, FORALL_PROD]
+    >> gvs []
+    >> imp_res_tac mem_load_flds_eq
+    >> first_x_assum (drule_at (Pat `mem_loads _ _ _ _ _ = SOME _`))
+    >> simp []
+    >> dep_rewrite.DEP_REWRITE_TAC [REWRITE_RULE [EVERY_MEM] dropWhile_APPEND_EVERY]
+    >> simp [MEM_MAP, PULL_EXISTS, FORALL_PROD]
+    >> impl_tac
+    >- (
+      imp_res_tac struct_infos_ok_append
+      >> simp []
+      >> rfs [struct_infos_ok_def]
+      >> rpt (first_x_assum (qspec_then `LENGTH xs1` mp_tac))
+      >> simp [EL_APPEND2, EL_APPEND1, DROP_APPEND2]
+    )
+    >> strip_tac
+    >> simp []
+    >> simp [LIST_EQ_REWRITE, EL_MAP, EL_ZIP]
+  )
+  >- (
+    gvs [compile_shape_def, mem_load_def, convert_v_def, v_flds_ok_def]
+  )
+  >- (
+    gvs [compile_shape_def, convert_v_def, v_flds_ok_def]
+    >> fs [cj 3 mem_load_def, option_case_eq]
+    >> rpt (first_x_assum drule)
+    >> gvs []
+    >> simp [size_of_compile_shape]
+  )
+QED
+
+
+Theorem compile_exp_correct:
+  ∀s e ctxt v.
+  eval s e = SOME v ∧
+  MAP (\(nm, info). (nm, info.fields)) s.structs = ctxt.structs ∧
+  FEVERY (\(nm, v). v_flds_ok ctxt.structs v) s.locals ∧
+  FEVERY (\(nm, v). v_flds_ok ctxt.structs v) s.globals ∧
+  structs_ok ctxt.structs
+  ⇒
+  v_flds_ok ctxt.structs v ∧ 
+  eval (convert_s s) (compile_exp ctxt e) = SOME (convert_v v)
+
+Proof
+
   recInduct (name_ind_cases [] eval_ind) >> rpt conj_tac
   >> rpt (gen_tac ORELSE disch_tac)
   >~ [`NStruct`]
   >- (
-    fs [eval_def, UNCURRY_EQ] \\ fs []
+    fs [eval_def, UNCURRY_EQ]
+    >> fs [option_case_eq, UNCURRY_EQ, UNZIP_MAP]
+    >> simp [compile_exp_def, eval_def, convert_v_def]
+    >> gvs [v_flds_ok_def]
+    >> qpat_x_assum `MAP _ _ = _.structs` (assume_tac o GSYM)
+    >> fs [ALOOKUP_MAP]
+    >> imp_res_tac opt_mmap_length_eq >> fs []
+    >> csimp [LIST_EQ_REWRITE, EL_MAP, EL_ZIP]
+    >> simp [SF ETA_ss]
+    >> conj_tac
+    >- (
+      ONCE_REWRITE_TAC [ELIM_UNCURRY]
+      >> simp [every_zip_snd]
+      >> drule_then (irule_at Any) opt_mmap_eq_every
+      >> simp []
+      >> metis_tac []
+    )
+    >> imp_res_tac alookup_map_structs_ok
+    >> simp [fields_in_order_reorder_noop]
+    >> simp [GSYM MAP_MAP_o, GSYM compile_exps_eq_map]
+    >> fs [SF ETA_ss]
+    >> dxrule compile_exp_correct_mmap_helper
+    >> simp [convert_v_def, LIST_EQ_REWRITE, EL_MAP, EL_ZIP]
+  )
+  >~ [`NField`]
+  >- (
+    fs [eval_def, option_case_eq, bool_case_eq, v_case_eq, compile_exp_def]
+    >> subgoal `old_exp_shape ctxt e = shape_of (THE (eval s e))`
+    >- cheat
+    >> simp [shape_of_def, convert_v_def]
+    >> Cases_on `ALOOKUP s.structs nm` >> fs []
+    >> qpat_x_assum `MAP _ _ = _.structs` (assume_tac o GSYM)
+    >> simp [alistTheory.ALOOKUP_MAP_2]
+    >> first_x_assum (drule_at (Pat `FEVERY _ _`))
+    >> simp [v_flds_ok_def, ALOOKUP_MAP_2]
+    >> strip_tac
+    >> drule_then drule map_fst_eq_alookup
+    >> strip_tac
+    >> fs [EL_MAP, EVERY_EL, convert_v_def]
+    >> res_tac
+    >> fs [ELIM_UNCURRY]
+  )
+  >~ [`Load`]
+  >- (
+    gvs [eval_def, option_case_eq, v_case_eq, word_lab_case_eq, compile_exp_def,
+        is_wf_shape_v_def, convert_v_def]
+    >> simp [convert_s_def, is_wf_shape_nil_compile_shape]
+
+mem_load_def
+
+word_lab_case_eq
+ 
+
+MEM_SPLIT_APPEND_first
+
+print_match [] ``afindi``
+
+DB.apropos ``MEM _ _`` |> DB.apropos_in ``(++)``
+
+    >> imp_res_tac ALOOKUP_MEM
+ 
+  >~ [`RStruct`]
+  >- (
+    gvs [eval_def, compile_exp_def, convert_v_def, v_flds_ok_def, option_case_eq]
+    >> fs [SF ETA_ss]
+    >> drule_then (irule_at Any) opt_mmap_eq_every
+    >> drule_then (irule_at Any) compile_exp_correct_mmap_helper
+    >> simp [SF SFY_ss]
+  )
+  >~ [`RField`]
+  >- (
+    gvs [eval_def, option_case_eq, v_case_eq, compile_exp_def]
+    >> fs [EVERY_EL, convert_v_def, EL_MAP, v_flds_ok_def]
+  )
+  >~ [`Panop`]
+  >- (
+    gvs [eval_def, option_case_eq, v_case_eq, compile_exp_def]
+    >> fs [convert_v_def, v_flds_ok_def, SF ETA_ss]
+    >> drule_then (simp o single) compile_exp_correct_mmap_helper
+    >> imp_res_tac every_convert_v_eq
+    >> fs []
+  )
+  >~ [`Op`]
+  >- (
+    gvs [eval_def, option_case_eq, v_case_eq, compile_exp_def]
+    >> fs [convert_v_def, v_flds_ok_def, SF ETA_ss]
+    >> drule_then (simp o single) compile_exp_correct_mmap_helper
+    >> imp_res_tac every_convert_v_eq
+    >> fs []
+  )
+
+
+
+  >> TRY (all_tac
+  >> gvs [eval_def, compile_exp_def, convert_v_def, v_flds_ok_def,
+    convert_s_def, FLOOKUP_FMAP_MAP2, AllCaseEqs ()]
+  >> simp [compile_exp_correct_mmap_helper, EL_MAP]
+  >> drule_then drule FEVERY_FLOOKUP
+  >> simp []
+  >> NO_TAC)
+
+
+
+  >- (
+    gvs [eval_def, option_case_eq, v_case_eq, compile_exp_def]
+    >> fs [EVERY_EL, convert_v_def, EL_MAP, v_flds_ok_def, SF ETA_ss]
+    >> drule_then (simp o single) compile_exp_correct_mmap_helper
+ 
+    >> simp [compile_exp_correct_mmap_helper, SF SFY_ss]
+    >> drule_then (irule_at Any) compile_exp_correct_mmap_helper
+    
+
+    >> fs [EVERY_EL, convert_v_def, EL_MAP, v_flds_ok_def]
+
+  >> TRY (all_tac
+  >> gvs [eval_def, compile_exp_def, convert_v_def, v_flds_ok_def,
+    convert_s_def, FLOOKUP_FMAP_MAP2, AllCaseEqs ()]
+  >> imp_res_tac every_convert_v_eq
+  >> simp [compile_exp_correct_mmap_helper, EL_MAP]
+  >> drule_then drule FEVERY_FLOOKUP
+  >> simp []
+  >> NO_TAC)
+
+print_find "fst_zip"
+print_find "map_fst"
+print_find "flookup_fmap"
+
+print_match [] ``ALOOKUP (MAP _ _)``;
+fs [Q.ISPEC `MAP _ _` EQ_SYM_EQ |> Q.SPEC `_.structs`]
+print_find "comm"
+EQ_COMM
+
+print_find "opt_mmap_el";
+
   )
   >~ [`NField`]
   >- (
